trying to prove transitivity of lr_refines by changing the quantifier rules to add taus

theories/Ref/LetRecRefines.v
@@ -42,6 +42,20 @@ Local Open Scope entree_scope.
 Definition SpecM' (E:EncType) stack A : Type :=
   entree_spec' (FunStackE E stack) A.
 
+(* Destruct an equality on VisF constructors into a dependent equality *)
+(* FIXME: move to SpecM.v *)
+Lemma injection_VisF_eq {E} `{EncodingType E} {R F} {e1 e2 : E}
+  {k1 : encodes e1 -> F} {k2 : encodes e2 -> F} :
+  VisF (R:=R) e1 k1 = VisF e2 k2 ->
+  existT (fun e => encodes e -> F) e1 k1 = existT _ e2 k2.
+Proof.
+  intro e. inversion e. reflexivity.
+Qed.
+
+Ltac observe_tau :=
+  (lazymatch goal with
+   | |- context F [TauF ?e] => replace (TauF e) with (observe (Tau e)); [ | reflexivity ]
+   end).
 
 Section lr_refines.
 
@@ -75,19 +89,19 @@ Inductive lr_refinesF (sim : SpecM E1 stk1 R1 -> SpecM E2 stk2 R2 -> Prop) : Spe
                             lr_refinesF sim ot1 (TauF t2)
 
 (* (forall a, t1 |= k a) => t1 |= Forall k *)
-| lr_refinesF_forallR A ot1 k : (forall a, lr_refinesF sim ot1 (observe (k a))) ->
+| lr_refinesF_forallR A ot1 k : (forall a, lr_refinesF sim ot1 (TauF (k a))) ->
                                 lr_refinesF sim ot1 (VisF (Spec_forall A) k)
 
 (* (exists a, t1 |= k a) => t1 |= Exists k *)
-| lr_refinesF_existsR A ot1 k a : lr_refinesF sim ot1 (observe (k a)) ->
+| lr_refinesF_existsR A ot1 k a : lr_refinesF sim ot1 (TauF (k a)) ->
                                   lr_refinesF sim ot1 (VisF (Spec_exists A) k)
 
 (* (exists a, k a |= t2) => Forall k |= t2 *)
-| lr_refinesF_forallL A ot2 k a : lr_refinesF sim (observe (k a)) ot2 ->
+| lr_refinesF_forallL A ot2 k a : lr_refinesF sim (TauF (k a)) ot2 ->
                                   lr_refinesF sim (VisF (Spec_forall A) k) ot2
 
 (* (forall a, k a |= t2) => Exists k |= t2 *)
-| lr_refinesF_existsL A ot2 k : (forall a, lr_refinesF sim (observe (k a)) ot2) ->
+| lr_refinesF_existsL A ot2 k : (forall a, lr_refinesF sim (TauF (k a)) ot2) ->
                                 lr_refinesF sim (VisF (Spec_exists A) k) ot2
 
 (* apply funs1 call1 >>= k1 |= t2 => CallS call1 >>= k1 |= t2 *)
@@ -146,15 +160,27 @@ Proof.
   subst. auto.
 Qed.
 
+(*
+(* Restatement of a helper lemma about normal refinement *)
+Lemma refinesF_TauR_inv_r' E1 E2 `{EncodingType E1} `{EncodingType E2}
+  (RPre : Rel E1 E2) (RPost : PostRel E1 E2) R1 R2 (RR : Rel R1 R2) r t1 t2 :
+  refinesF RPre RPost RR (upaco2 (refines_ RPre RPost RR) r) (observe t1) (TauF t2) ->
+  refinesF RPre RPost RR (upaco2 (refines_ RPre RPost RR) r) (observe t1) (observe t2).
+Proof.
+  intro. remember (TauF t2) as x.
+  remember (observe t1) as ot1; clear Heqot1.
+  induction H1; inversion Heqx.
+  - constructor. pstep_reverse.
 
-
-Section lr_refines_props.
-
-Context {E1 E2 : EncType} {stk1 stk2 : FunStack} {R1 R2 : Type} {RR : Rel R1 R2}.
-Context (funs1 : FrameTuple E1 stk1) (funs2 : FrameTuple E2 stk2).
+induction H1.
+  intros. induction H1
+  intros. pstep_reverse. apply refines_TauR_inv. pstep. auto.
+Qed.
+*)
 
 (* Lift a relation on FunStackE events from the nil stack to arbitrary ones *)
-Definition liftNilRel (R : Rel (FunStackE E1 pnil) (FunStackE E2 pnil)) :
+Definition liftNilRel {E1 E2 stk1 stk2}
+  (R : Rel (FunStackE E1 pnil) (FunStackE E2 pnil)) :
   Rel (FunStackE E1 stk1) (FunStackE E2 stk2) :=
   fun e1 e2 => match e1,e2 with
                | inr e1', inr e2' => R (inr e1') (inr e2')
@@ -162,12 +188,371 @@ Definition liftNilRel (R : Rel (FunStackE E1 pnil) (FunStackE E2 pnil)) :
                end.
 
 (* Lift a postcondition on FunStackE events from the nil stack to arbitrary ones *)
-Definition liftNilPostRel (R : PostRel (FunStackE E1 pnil) (FunStackE E2 pnil)) :
+Definition liftNilPostRel {E1 E2 stk1 stk2}
+  (R : PostRel (FunStackE E1 pnil) (FunStackE E2 pnil)) :
   PostRel (FunStackE E1 stk1) (FunStackE E2 stk2) :=
   fun e1 e2 => match e1,e2 with
                | inr e1', inr e2' => R (inr e1') (inr e2')
                | _,_ => fun _ _ => False
                end.
+
+(* Compose two liftNilRel proofs *)
+Lemma liftNilRel_compose {E1 E2 E3 stk1 stk2 stk3} R12 R23 x y z :
+  @liftNilRel E1 E2 stk1 stk2 R12 x y ->
+  @liftNilRel E2 E3 stk2 stk3 R23 y z ->
+  liftNilRel (rcompose R12 R23) x z.
+Proof.
+  intros. destruct x; destruct y; destruct z; cbn in *; try contradiction.
+  eexists; split; eassumption.
+Qed.
+
+Lemma elim_RComposePostRel {E1 E2 E3} `{EncodingType E1} `{EncodingType E2}
+  `{EncodingType E3} (R1 : Rel E1 E2) (R2 : Rel E2 E3) RPost1 RPost2
+  a b c x z :
+  R1 a b -> R2 b c ->
+  RComposePostRel R1 R2 RPost1 RPost2 a c x z ->
+  exists y, RPost1 a b x y /\ RPost2 b c y z.
+Proof.
+  intros. destruct H4. apply H4; assumption.
+Qed.
+
+(* Destruct the composition of two liftNilPostRel proofs *)
+Lemma liftNilPostRel_compose_elim {E1 E2 E3 stk1 stk2 stk3} R12 R23 RPost12 RPost23
+  (e1 : FunStackE E1 stk1) (e2 : FunStackE E2 stk2) (e3 : FunStackE E3 stk3) x z :
+  liftNilRel R12 e1 e2 -> liftNilRel R23 e2 e3 ->
+  liftNilPostRel (RComposePostRel R12 R23 RPost12 RPost23) e1 e3 x z ->
+  exists y:encodes e2,
+    liftNilPostRel RPost12 e1 e2 x y /\ liftNilPostRel RPost23 e2 e3 y z.
+Proof.
+  intros. destruct e1; destruct e2; destruct e3; cbn in *; try contradiction.
+  destruct (elim_RComposePostRel _ _ _ _ _ _ _ _ _ H H0 H1). destruct H2.
+  eexists; split; eassumption.
+Qed.
+
+
+(*** Inversion lemmas about refinement ***)
+Section lr_refines_inv.
+Context {E1 E2 : EncType} {stk1 stk2 : FunStack} {R1 R2 : Type}.
+Context (funs1 : FrameTuple E1 stk1) (funs2 : FrameTuple E2 stk2).
+
+Context (RPre : Rel (FunStackE E1 stk1) (FunStackE E2 stk2))
+  (RPost : PostRel (FunStackE E1 stk1) (FunStackE E2 stk2))
+  (RR : R1 -> R2 -> Prop).
+
+Lemma lr_refines_TauL_inv t1 t2 :
+  lr_refines funs1 funs2 RPre RPost RR (Tau t1) t2 ->
+  lr_refines funs1 funs2 RPre RPost RR t1 t2.
+Proof.
+  remember (TauF t1) as x.
+  intro. punfold H. red in H. simpl in H. pfold. red.
+  remember (observe t2) as ot2.
+  clear t2 Heqot2.
+  induction H; inversion Heqx.
+  - pclearbot. constructor. pstep_reverse. rewrite <- H1.
+    eapply paco2_mon; [ eassumption | ]. intros x0 x1 b; destruct b.
+  - rewrite <- H1. eapply monotone_lr_refinesF; [ | eassumption ].
+    intros. pclearbot. left. eapply paco2_mon; [ eassumption | ].
+    intros. contradiction.
+  - constructor. apply IHlr_refinesF. assumption.
+  - constructor. intros. apply H0. assumption.
+  - econstructor. apply IHlr_refinesF. assumption.
+  - constructor. apply IHlr_refinesF. assumption.
+Qed.
+
+Lemma lr_refines_TauR_inv t1 t2 :
+  lr_refines funs1 funs2 RPre RPost RR t1 (Tau t2) ->
+  lr_refines funs1 funs2 RPre RPost RR t1 t2.
+Proof.
+  remember (TauF t2) as x.
+  intro. punfold H. red in H. simpl in H. pfold. red.
+  remember (observe t1) as ot1. clear t1 Heqot1.
+  induction H; inversion Heqx.
+  - pclearbot. constructor. pstep_reverse. rewrite <- H1.
+    eapply paco2_mon; [ eassumption | ]. intros x0 x1 b; destruct b.
+  - constructor. apply IHlr_refinesF. assumption.
+  - rewrite <- H1. eapply monotone_lr_refinesF; [ | eassumption ].
+    intros. pclearbot. left. eapply paco2_mon; [ eassumption | ].
+    intros. contradiction.
+  - econstructor. apply IHlr_refinesF. assumption.
+  - constructor. intros. apply H0. assumption.
+  - constructor. apply IHlr_refinesF. assumption.
+Qed.
+
+Lemma lr_refinesF_TauR_inv t1 t2 :
+  lr_refinesF funs1 funs2 RPre RPost RR (upaco2 (lr_refines_ funs1 funs2 RPre RPost RR) bot2) (observe t1) (TauF t2) ->
+  lr_refinesF funs1 funs2 RPre RPost RR (upaco2 (lr_refines_ funs1 funs2 RPre RPost RR) bot2) (observe t1) (observe t2).
+Proof.
+  intros. pstep_reverse. apply lr_refines_TauR_inv. pstep. apply H.
+Qed.
+
+Lemma lr_refinesF_TauL_inv t1 t2 :
+  lr_refinesF funs1 funs2 RPre RPost RR
+    (upaco2 (lr_refines_ funs1 funs2 RPre RPost RR) bot2) (TauF t1) (observe t2) ->
+  lr_refinesF funs1 funs2 RPre RPost RR
+    (upaco2 (lr_refines_ funs1 funs2 RPre RPost RR) bot2) (observe t1) (observe t2).
+Proof.
+  intros. pstep_reverse. apply lr_refines_TauL_inv. pstep. assumption.
+Qed.
+
+Lemma lr_refines_forallR_inv A t1 k2 :
+  lr_refines funs1 funs2 RPre RPost RR
+    t1 (Vis (@Spec_forall (FunStackE E2 stk2) A) k2) ->
+  forall a, lr_refines funs1 funs2 RPre RPost RR t1 (Tau (k2 a)).
+Proof.
+  intros ref12 a. punfold ref12. red in ref12. cbn in ref12. pstep. red.
+  remember (observe t1) as ot1; clear t1 Heqot1.
+  remember (VisF (Spec_forall A) k2) as ot2.
+  induction ref12; try discriminate.
+  - apply lr_refinesF_TauL. apply IHref12. assumption.
+  - inversion Heqot2. revert k Heqot2 H H0 H3; rewrite H2; intros.
+    inj_existT. rewrite H3 in H. apply H.
+  - eapply lr_refinesF_forallL. apply IHref12. assumption.
+  - apply lr_refinesF_existsL. intros. apply H0. assumption.
+  - apply lr_refinesF_unfoldL. apply IHref12. assumption.
+Qed.
+
+
+Lemma lr_refines_existsL_inv A k1 t2 :
+  lr_refines funs1 funs2 RPre RPost RR
+    (Vis (@Spec_exists (FunStackE E1 stk1) A) k1) t2 ->
+  forall a, lr_refines funs1 funs2 RPre RPost RR (Tau (k1 a)) t2.
+Proof.
+  intros ref12 a. punfold ref12. red in ref12. cbn in ref12. pstep. red.
+  remember (observe t2) as ot2; clear t2 Heqot2.
+  remember (VisF (Spec_exists A) k1) as ot1.
+  induction ref12; try discriminate.
+  - apply lr_refinesF_TauR. apply IHref12. assumption.
+  - apply lr_refinesF_forallR. intros. apply H0. assumption.
+  - eapply lr_refinesF_existsR. apply IHref12. assumption.
+  - inversion Heqot1. revert k Heqot1 ot2 H a H0 H3; rewrite H2; intros.
+    inj_existT. rewrite H3 in H. apply H.
+  - apply lr_refinesF_unfoldR. apply IHref12. assumption.
+Qed.
+
+
+(* A version of lr_refinesF specialized to a forall on the left *)
+Inductive forallLRRefinesF (sim : SpecM E1 stk1 R1 -> SpecM E2 stk2 R2 -> Prop)
+  {A : QuantEnc} (k1 : encodes A -> SpecM E1 stk1 R1) : SpecM' E2 stk2 R2 -> Prop :=
+  | forallLRRefines_forallR (B : QuantEnc) k2 :
+    (forall b, forallLRRefinesF sim k1 (TauF (k2 b))) ->
+    forallLRRefinesF sim k1 (VisF (Spec_forall B) k2)
+  | forallLRRefines_forallL t (a : encodes A) :
+    lr_refinesF funs1 funs2 RPre RPost RR sim (TauF (k1 a)) t ->
+    forallLRRefinesF sim k1 t
+  | forallLRRefines_existsR B k2 (b : encodes B) :
+    forallLRRefinesF sim k1 (TauF (k2 b)) ->
+    forallLRRefinesF sim k1 (VisF (Spec_exists B : SpecEvent (FunStackE _ _)) k2)
+  | forallLRRefines_TauR t2 :
+    forallLRRefinesF sim k1 (observe t2) ->
+    forallLRRefinesF sim k1 (TauF t2)
+  | forallLRRefines_unfoldR call2 k2 :
+    forallLRRefinesF sim k1 (TauF (applyFrameTuple E2 stk2 funs2 call2 >>= k2)) ->
+    forallLRRefinesF sim k1 (VisF (Spec_vis (inl call2)) k2)
+.
+
+Lemma lr_refinesF_forallL_inv sim A k1 t2 :
+  lr_refinesF funs1 funs2 RPre RPost RR sim
+    (VisF (@Spec_forall (FunStackE E1 stk1) A) k1) t2 ->
+  forallLRRefinesF sim k1 t2.
+Proof.
+  intros. remember (VisF (Spec_forall A) k1) as ot1.
+  induction H; try discriminate.
+  - apply forallLRRefines_TauR; apply IHlr_refinesF; assumption.
+  - apply forallLRRefines_forallR; intros. apply H0. assumption.
+  - eapply forallLRRefines_existsR. apply IHlr_refinesF. assumption.
+  - inversion Heqot1. revert k Heqot1 a H IHlr_refinesF H2. rewrite H1. intros.
+    inj_existT. rewrite H2 in H. eapply forallLRRefines_forallL. apply H.
+  - apply forallLRRefines_unfoldR. apply IHlr_refinesF. assumption.
+Qed.
+
+(* A version of lr_refinesF specialized to an exists on the right *)
+Inductive existsLRRefinesF (sim : SpecM E1 stk1 R1 -> SpecM E2 stk2 R2 -> Prop)
+  {A : QuantEnc} (k2 : encodes A -> SpecM E2 stk2 R2) : SpecM' E1 stk1 R1 -> Prop :=
+  | existsLRRefines_existsR t (a : encodes A) :
+    lr_refinesF funs1 funs2 RPre RPost RR sim t (TauF (k2 a)) ->
+    existsLRRefinesF sim k2 t
+  | existsLRRefines_forallL B k1 (b : encodes B) :
+    existsLRRefinesF sim k2 (TauF (k1 b)) ->
+    existsLRRefinesF sim k2 (VisF (Spec_forall B : SpecEvent (FunStackE _ _)) k1)
+  | existsLRRefines_existsL (B : QuantEnc) k1 :
+    (forall b, existsLRRefinesF sim k2 (TauF (k1 b))) ->
+    existsLRRefinesF sim k2 (VisF (Spec_exists B) k1)
+  | existsLRRefines_TauL t1 :
+    existsLRRefinesF sim k2 (observe t1) ->
+    existsLRRefinesF sim k2 (TauF t1)
+  | existsLRRefines_unfoldL call1 k1 :
+    existsLRRefinesF sim k2 (TauF (applyFrameTuple E1 stk1 funs1 call1 >>= k1)) ->
+    existsLRRefinesF sim k2 (VisF (Spec_vis (inl call1)) k1)
+.
+
+Lemma lr_refinesF_existsR_inv sim A t1 k2 :
+  lr_refinesF funs1 funs2 RPre RPost RR sim
+    t1 (VisF (@Spec_exists (FunStackE E2 stk2) A) k2) ->
+  existsLRRefinesF sim k2 t1.
+Proof.
+  intros. remember (VisF (Spec_exists A) k2) as ot2.
+  induction H; try discriminate.
+  - apply existsLRRefines_TauL; apply IHlr_refinesF; assumption.
+  - inversion Heqot2. revert k Heqot2 a H IHlr_refinesF H2; rewrite H1; intros.
+    inj_existT. rewrite H2 in H. eapply existsLRRefines_existsR. apply H.
+  - eapply existsLRRefines_forallL. apply IHlr_refinesF. assumption.
+  - apply existsLRRefines_existsL. intros. apply H0. assumption.
+  - apply existsLRRefines_unfoldL. apply IHlr_refinesF. assumption.
+Qed.
+
+Lemma lr_refines_callL_inv pre post call1 k1 t2 :
+  lr_refines funs1 funs2 (liftNilRel pre) (liftNilPostRel post) RR
+    (Vis (Spec_vis (inl call1)) k1) t2 ->
+  lr_refines funs1 funs2 (liftNilRel pre) (liftNilPostRel post) RR
+    (Tau (applyFrameTuple E1 stk1 funs1 call1 >>= k1)) t2.
+Proof.
+  intros ref12. punfold ref12. red in ref12. cbn in ref12. pstep. red.
+  remember (observe t2) as ot2; clear t2 Heqot2.
+  remember (VisF (Spec_vis (inl call1)) k1) as ot1.
+  induction ref12; try discriminate.
+  - inversion Heqot1. rewrite H2 in H. destruct e2; destruct H.
+  - apply lr_refinesF_TauR. apply IHref12. assumption.
+  - apply lr_refinesF_forallR; intros. apply H0. assumption.
+  - eapply lr_refinesF_existsR. apply IHref12. assumption.
+  - inversion Heqot1. revert k0 Heqot1 ref12 IHref12. rewrite H0. intros.
+    remember (injection_VisF_eq Heqot1) as e. clear Heqe. inj_existT.
+    rewrite <- e. apply ref12.
+  - apply lr_refinesF_unfoldR. apply IHref12. assumption.
+Qed.
+
+
+End lr_refines_inv.
+
+
+
+(*** Proving transitivity ***)
+
+Lemma lr_refines_trans {E1 E2 E3} {stk1 stk2 stk3} {R1 R2 R3}
+  RPre1 RPre2 RPost1 RPost2
+  (RR1 : R1 -> R2 -> Prop) (RR2 : R2 -> R3 -> Prop)
+  (funs1 : FrameTuple E1 stk1) (funs2 : FrameTuple E2 stk2)
+  (funs3 : FrameTuple E3 stk3)
+  (t1 : SpecM E1 stk1 R1) (t2 : SpecM E2 stk2 R2) (t3 : SpecM E3 stk3 R3) :
+  lr_refines funs1 funs2 (liftNilRel RPre1) (liftNilPostRel RPost1) RR1 t1 t2 ->
+  lr_refines funs2 funs3 (liftNilRel RPre2) (liftNilPostRel RPost2) RR2 t2 t3 ->
+  lr_refines funs1 funs3 (liftNilRel (rcompose RPre1 RPre2))
+    (liftNilPostRel (RComposePostRel RPre1 RPre2 RPost1 RPost2))
+    (rcompose RR1 RR2) t1 t3.
+Proof.
+  revert t1 t2 t3; pcofix CIH; intros t1 t2 t3 ref12 ref23.
+  pfold. red. punfold ref12. red in ref12. punfold ref23. red in ref23.
+  remember (observe t1) as ot1. clear t1 Heqot1.
+  remember (observe t2) as ot2. clear t2 Heqot2.
+  revert t3 ref23; induction ref12; intros.
+  - remember (RetF r2) as x. induction ref23; inversion Heqx.
+    + constructor. exists r2; split; [ assumption | ].
+      rewrite <- H2. assumption.
+    + constructor. apply IHref23. assumption.
+    + constructor. intros. apply H1. assumption.
+    + econstructor. apply IHref23. assumption.
+    + constructor. apply IHref23. assumption.
+  - pclearbot.
+    assert (lr_refines funs2 funs3 (liftNilRel RPre2) (liftNilPostRel RPost2) RR2 t2 t3) as ref23'.
+    { apply lr_refines_TauL_inv. pstep. assumption. }
+    clear ref23. punfold ref23'. red in ref23'.
+    remember (observe t3) as ot3; clear t3 Heqot3.
+    punfold H. red in H.
+    remember (observe t2) as ot2. clear t2 Heqot2.
+    revert t1 H. induction ref23'; intros.
+    + apply lr_refinesF_TauL.
+      (* Proof that  t1 |= Ret r1 |= Ret r2  implies Tau t1 |= Ret r2 *)
+      remember (observe t1) as ot1; clear t1 Heqot1.
+      remember (RetF r1) as ot0. induction H0; try discriminate Heqot0.
+      * inversion Heqot0. apply lr_refinesF_Ret. rewrite H2 in H0.
+        eexists; split; eassumption.
+      * apply lr_refinesF_TauL. apply IHlr_refinesF. assumption.
+      * eapply lr_refinesF_forallL. apply IHlr_refinesF. assumption.
+      * apply lr_refinesF_existsL. intros. apply H1. assumption.
+      * apply lr_refinesF_unfoldL. apply IHlr_refinesF. assumption.
+    + apply lr_refinesF_Tau. right. pclearbot. eapply CIH; [ | eassumption ].
+      apply lr_refines_TauR_inv. pstep. apply H0.
+    + apply lr_refinesF_TauL.
+      (* Proof tht  t1 |= Vis e2 k2 |= Vis e3 k3  implies t1 |= Vis e3 k3 *)
+      remember (observe t1) as ot1; clear t1 Heqot1.
+      remember (VisF (Spec_vis e1) k1) as ot0.
+      induction H1; try discriminate Heqot0.
+      * set (e := injection_VisF_eq Heqot0). inversion e.
+        revert k3 Heqot0 H1 H2 e; rewrite H4; intros. clear e3 H4. inj_existT.
+        apply lr_refinesF_Vis; [ eapply liftNilRel_compose; eassumption | ].
+        intros.
+        destruct (liftNilPostRel_compose_elim _ _ _ _ _ _ _ _ _ H1 H H3)
+          as [ c [ PR_ac PR_cb ]].
+        remember (H2 a c PR_ac) as ref_k0_k3. clear Heqref_k0_k3.
+        rewrite <- e in H0.
+        remember (H0 c b PR_cb) as ref_k3_k2. clear Heqref_k3_k2.
+        pclearbot.
+        right. eapply CIH; eassumption.
+      * apply lr_refinesF_TauL. apply IHlr_refinesF. assumption.
+      * eapply lr_refinesF_forallL. apply IHlr_refinesF. assumption.
+      * eapply lr_refinesF_existsL. intros. apply H2. assumption.
+      * apply lr_refinesF_unfoldL. apply IHlr_refinesF. assumption.
+      * inversion Heqot0. rewrite <- H3 in H. destruct e2; simpl in H; contradiction.
+    + apply IHref23'. pstep_reverse. apply lr_refines_TauR_inv.
+      pstep. apply H.
+    + apply lr_refinesF_Tau. right.
+      apply (CIH _ (go _ _ ot1)); pstep; assumption.
+    + apply lr_refinesF_forallR. intros. apply H0. assumption.
+    + eapply lr_refinesF_existsR. apply IHref23'. assumption.
+    + apply IHref23'. observe_tau. pstep_reverse.
+      apply lr_refines_forallR_inv. pstep. apply H.
+    + assert (existsLRRefinesF funs1 funs2
+                (liftNilRel RPre1) (liftNilPostRel RPost1) RR1
+                (upaco2 (lr_refines_ funs1 funs2
+                           (liftNilRel RPre1) (liftNilPostRel RPost1) RR1) bot2)
+                k (observe t1))
+        as ref_exR;
+        [ apply lr_refinesF_existsR_inv; assumption | ].
+      clear H1. remember (observe t1) as ot1.
+      assert (t1 = go _ _ ot1); [ destruct t1; rewrite Heqot1; reflexivity | ].
+      subst t1. clear Heqot1.
+      induction ref_exR; intros.
+      * apply (H0 a). assumption.
+      * 
+admit. (* Need inversion lemma on t1 |= exists k *)
+    + apply IHref23'.
+      admit. (* t1 |= Vis call k1  implies t1 |= Tau (unfold call >>= k1) *)
+    + apply lr_refinesF_unfoldR. apply IHref23'. assumption.
+  - admit. (* Vis e1 k1 |= Vis e2 k2 |= t3  implies Vis e1 k1 |= t3 *)
+  - apply lr_refinesF_TauL. apply IHref12. assumption.
+  - apply IHref12. pstep_reverse. apply lr_refines_TauL_inv. pstep. assumption.
+  - assert (forallLRRefinesF funs2 funs3
+              (liftNilRel RPre2) (liftNilPostRel RPost2) RR2
+              (upaco2 (lr_refines_ funs2 funs3
+                         (liftNilRel RPre2) (liftNilPostRel RPost2) RR2) bot2)
+              k
+              (observe t3))
+      as ref_allL;
+      [ apply lr_refinesF_forallL_inv; assumption | ].
+    clear ref23. remember (observe t3) as ot3; clear t3 Heqot3.
+    induction ref_allL.
+    + apply lr_refinesF_forallR; intros. apply H2.
+    + apply (H0 a (go _ _ t)). apply H1.
+    + eapply lr_refinesF_existsR. apply IHref_allL.
+    + apply lr_refinesF_TauR. apply IHref_allL.
+    + apply lr_refinesF_unfoldR. apply IHref_allL.
+  - apply IHref12. observe_tau.
+    pstep_reverse. apply lr_refines_existsL_inv. pstep. apply ref23.
+  - eapply lr_refinesF_forallL. apply IHref12. assumption.
+  - apply lr_refinesF_existsL. intros. apply H0. assumption.
+  - apply lr_refinesF_unfoldL. apply IHref12. assumption.
+  - apply IHref12. observe_tau. pstep_reverse.
+    apply lr_refines_callL_inv. pstep. assumption.
+Admitted.
+
+
+(*** Proving other properties ***)
+
+
+Section lr_refines_props.
+
+Context {E1 E2 : EncType} {stk1 stk2 : FunStack} {R1 R2 : Type} {RR : Rel R1 R2}.
+Context (funs1 : FrameTuple E1 stk1) (funs2 : FrameTuple E2 stk2).
+
 
 Lemma observing_LetRecS E R stk funs body :
   LetRecS E R stk funs body = LetRecS E R stk funs (go _ _ (observe body)).
@@ -181,6 +566,7 @@ Proof.
   reflexivity.
 Qed.
 
+(*
 (* lr_refines is sound, meaning that it implies two letrecs refine each other *)
 Lemma lr_refines_soundness RPre RPost t1 t2 :
   lr_refines funs1 funs2 (liftNilRel RPre) (liftNilPostRel RPost) RR t1 t2 ->
@@ -203,13 +589,15 @@ Proof.
     destruct (H0 a b H1); [ | destruct H2 ]. apply H2.
   - cbn. apply refinesF_TauL. apply IHlr_refinesF. intros. apply CIH. assumption.
   - cbn. apply refinesF_TauR. apply IHlr_refinesF. intros. apply CIH. assumption.
-  - cbn. apply refinesF_forallR. intros. apply H0. intros. apply CIH. assumption.
+  - cbn. apply refinesF_forallR. intros.
+    apply H0. intros. apply CIH. assumption.
   - cbn. eapply refinesF_existsR. apply IHlr_refinesF.
     intros. apply CIH. assumption.
   - cbn. eapply refinesF_forallL. apply IHlr_refinesF.
     intros. apply CIH. assumption.
   - cbn. apply refinesF_existsL. intros. apply H0. intros. apply CIH. assumption.
 Qed.
+*)
 
 (* lr_refines is complete, meaning that it holds whenever two letrecs refine
 each other *)
@@ -223,7 +611,7 @@ Proof.
   punfold H2. red in H2. pstep. red.
   remember (observe t1') as ot1'. remember (observe t2') as ot2'.
   clear t1' Heqot1' t2' Heqot2'.
-  hinduction H2 before r; intros; pclearbot; eauto.
+  hinduction H2 before r; intros; pclearbot.
   - destruct t1 as [[]]; destruct t2 as [[]]; try discriminate.
     + injection H0; intros; injection H1; intros. constructor.
       subst r1. subst r2. assumption.
@@ -276,17 +664,41 @@ Proof.
     destruct u; [ assumption | destruct b0 ].
   - pstep. apply lr_refinesF_TauL. pstep_reverse.
   - pstep. apply lr_refinesF_TauR. pstep_reverse.
-  - pstep. apply lr_refinesF_forallR. intros. pstep_reverse. apply H0.
-  - pstep. eapply lr_refinesF_existsR. pstep_reverse. apply IHmref.
-  - pstep. eapply lr_refinesF_forallL. pstep_reverse. apply IHmref.
-  - pstep. apply lr_refinesF_existsL. intros. pstep_reverse. apply H0.
+  - pstep. apply lr_refinesF_forallR. intros.
+    change
+      (lr_refinesF funs1 funs2 RPre RPost RR
+         (upaco2 (lr_refines_ funs1 funs2 RPre RPost RR) r)
+         (observe (x <- go _ _ ot1;; k1 x))
+         (observe ((x <- Tau (k a);; k2 x)))).
+    pstep_reverse.
+  - pstep. apply (lr_refinesF_existsR _ _ _ _ _ _ _ _ _ a).
+    change
+      (lr_refinesF funs1 funs2 RPre RPost RR
+         (upaco2 (lr_refines_ funs1 funs2 RPre RPost RR) r)
+         (observe (x <- go _ _ ot1;; k1 x))
+         (observe ((x <- Tau (k a);; k2 x)))).
+    pstep_reverse.
+  - pstep. apply (lr_refinesF_forallL _ _ _ _ _ _ _ _ _ a).
+    change
+      (lr_refinesF funs1 funs2 RPre RPost RR
+         (upaco2 (lr_refines_ funs1 funs2 RPre RPost RR) r)
+         (observe ((x <- Tau (k a);; k1 x)))
+         (observe (x <- go _ _ ot2;; k2 x))).
+    pstep_reverse.
+  - pstep. apply lr_refinesF_existsL. intros.
+    change
+      (lr_refinesF funs1 funs2 RPre RPost RR
+         (upaco2 (lr_refines_ funs1 funs2 RPre RPost RR) r)
+         (observe ((x <- Tau (k a);; k1 x)))
+         (observe (x <- go _ _ ot2;; k2 x))).
+    pstep_reverse.
   - pstep. setoid_rewrite bind_vis. apply lr_refinesF_unfoldL.
     change
       (lr_refinesF funs1 funs2 RPre RPost RR
          (upaco2 (lr_refines_ funs1 funs2 RPre RPost RR) r)
          (observe (Tau (x <- applyFrameTuple E1 stk1 funs1 call1;; EnTree.bind (k0 x) k1)))
          (observe (x <- {| _observe := ot2 |};; k2 x))).
-    pstep_reverse. 
+    pstep_reverse.
     setoid_rewrite <- bind_tau. setoid_rewrite <- bind_bind.
     apply IHmref.
   - pstep. setoid_rewrite bind_vis. apply lr_refinesF_unfoldR.
